New abstraction

symbolic_execution.v
@@ -12,6 +12,12 @@ Inductive input_list : Type :=
 |EmptyList
 |ConsList (i : input) (s : input_list).
 
+Fixpoint list_size (l : input_list) : nat :=
+match l with
+|EmptyList => 0
+|ConsList i s => S (list_size s)
+end.
+
 Inductive conc_state : Type :=
 |EmptyState
 |ConsState (i: input) (s: state).
@@ -22,6 +28,16 @@ the concrete execution of ConcState A with an input  *)
 Definition concrete_execution := Ensemble conc_state -> input -> Ensemble conc_state.
 
 Axiom conc_ex : concrete_execution.
+
+(*Definition concrete_execution_n := Ensemble conc_state -> input -> Ensemble conc_state.
+
+Axiom conc_ex_n : concrete_execution_n.*)
+
+Fixpoint conc_ex_input_list (states : Ensemble conc_state) (ilist : input_list) : Ensemble conc_state:=
+match ilist with
+|EmptyList => states
+|ConsList inp list_last_elem => conc_ex_input_list (conc_ex states inp) list_last_elem
+end.
 
 
 
@@ -51,6 +67,10 @@ Axiom get_phi : get_sym_state.
 Definition get_path_constraint := sym_state -> PC.
 Axiom get_pc : get_path_constraint.
 
+Definition s_e := sym_state -> sym_state.
+Axiom sym_ex : s_e.
+
+
 
 Definition uni := Phi -> PC -> Ensemble ConcState.conc_state.
 Axiom concretize : uni.
@@ -61,6 +81,10 @@ Axiom get_input : get_inp.
 Inductive SE_tree : Type :=
 | leaf: SE_tree
 | ConsNode: SE_tree -> sym_state -> SE_tree -> SE_tree.
+
+Definition s_e_n := sym_state -> nat -> SE_tree.
+Axiom sym_ex_n : s_e_n.
+
 
 Definition root (t : SE_tree) : sym_state :=
 match t with 
@@ -145,11 +169,52 @@ match tlist with
 |h :: t => S (size h)
 end.
 
+
+
 Definition is_connected  (tlist : SE_tree_list) : Prop :=
  forall (A B : SE_tree),
  (size tlist) >= 2 ->
  (is_consecutive_in_order A B tlist) ->
   is_leaf_state A (root B). 
+
+
+
+
+Definition singleton (x : ConcState.conc_state) : Ensemble ConcState.conc_state :=
+Singleton ConcState.conc_state x.
+
+(*Axiom lem_1 : forall (conc1 conc2 : ConcState.conc_state) (inp1 : ConcState.input)
+ (sym1: SymbolicExec.sym_state),
+(conc_ex (singleton conc1) inp1 = (singleton conc2)) /\ (In ConcState.conc_state (concretize (get_phi sym1) (get_pc sym1)) conc1)  ->
+exists sym2, 
+(In ConcState.conc_state (concretize (get_phi sym2) (get_pc sym2)) conc2) /\ 
+(is_leaf_state (sym_ex_n sym1) sym2). *)
+
+Axiom lem_1_n : forall (conc1 conc2 : ConcState.conc_state) (inp1 : ConcState.input_list)
+ (sym1: SymbolicExec.sym_state) (n : nat),
+(list_size inp1 = n)/\(conc_ex_input_list (singleton conc1) inp1 = (singleton conc2)) /\ (In ConcState.conc_state (concretize (get_phi sym1) (get_pc sym1)) conc1)  ->
+exists sym2, 
+(In  ConcState.conc_state (concretize (get_phi sym2) (get_pc sym2)) conc2) /\ (is_leaf_state (sym_ex_n sym1 n) sym2).
+
+
+
+(*
+Axiom lem_2 : forall (conc2 : ConcState.conc_state) (inp1 : ConcState.input)
+ (sym1 sym2: SymbolicExec.sym_state),
+(in_tree (sym_ex_with_branching sym1) sym2) /\ (In ConcState.conc_state (concretize (get_phi sym2) (get_pc sym2)) conc2)  ->
+exists conc1, 
+(In ConcState.conc_state (concretize (get_phi sym1) (get_pc sym1)) conc1) /\ 
+((conc_ex (singleton conc1) inp1) = (singleton conc2)).*)
+
+Axiom lem_2_n : forall (conc2 : ConcState.conc_state)
+ (sym1 sym2: SymbolicExec.sym_state) (n:nat),
+(is_leaf_state (sym_ex_n sym1 n) sym2) /\ (In ConcState.conc_state (concretize (get_phi sym2) (get_pc sym2)) conc2)  ->
+exists conc1, exists inp1,
+(list_size inp1 = n) /\
+(In ConcState.conc_state (concretize (get_phi sym1) (get_pc sym1)) conc1) /\ 
+(conc_ex_input_list (singleton conc1) inp1 = (singleton conc2)).
+
+
 
 
 End SymbolicExec.
@@ -173,7 +238,75 @@ Definition circle_op_2 (sym : SymbolicExec.sym_state) : Ensemble ConcState.conc_
 concretize (get_phi sym) (get_pc sym).
 
 
+Definition trees_connect (A B : SE_tree) : Prop :=
+forall (x y : sym_state),
+(is_leaf_state A x) /\ (is_leaf_state B y) ->
+Included ConcState.conc_state 
+(circle_op_2 x)
+(circle_op_1 (root B) y).
+
+
+Definition is_connected2 (tlist : SE_tree_list) : Prop :=
+forall (A B : SE_tree),
+ (size tlist) >= 2 ->
+ (is_consecutive_in_order A B tlist) ->
+  trees_connect A B. 
+
+Theorem lem_1_n_circle_op_2 : forall (conc1 conc2 : ConcState.conc_state) (inp1 : ConcState.input_list)
+ (sym1: SymbolicExec.sym_state) (n : nat),
+(list_size inp1 = n)/\(conc_ex_input_list (singleton conc1) inp1 = (singleton conc2)) 
+/\ (In ConcState.conc_state (circle_op_2 sym1) conc1)  ->
+exists sym2, 
+(In  ConcState.conc_state (circle_op_2 sym2) conc2) /\ (is_leaf_state (sym_ex_n sym1 n) sym2).
+Proof. unfold circle_op_2. apply lem_1_n. Qed.
+
+
+Theorem lem_2_n_circle_op_2 : forall (conc2 : ConcState.conc_state)
+ (sym1 sym2: SymbolicExec.sym_state) (n:nat),
+(is_leaf_state (sym_ex_n sym1 n) sym2) /\ (In ConcState.conc_state (circle_op_2 sym2) conc2)  ->
+exists conc1, exists inp1,
+(list_size inp1 = n) /\
+(In ConcState.conc_state (circle_op_2 sym1) conc1) /\ 
+(conc_ex_input_list (singleton conc1) inp1 = (singleton conc2)).
+Proof. unfold circle_op_2. apply lem_2_n. Qed.
+
 Variable init_conc_states: Ensemble ConcState.conc_state.
+
+
+Axiom base_case: 
+forall s0 s : SE_tree,
+is_connected (([ ] :: s0) :: s) ->
+conc_ex
+  (conc_ex init_conc_states
+     (get_input (get_pc (root s0))))
+  (get_input (get_pc (root s))) =
+circle_op_2 (root s).
+
+Axiom bc2: 
+forall s0 s : SE_tree,
+is_connected2 (([ ] :: s0) :: s) ->
+forall c : sym_state,
+is_leaf_state s0 c ->
+conc_ex
+  (conc_ex init_conc_states
+     (get_input (get_pc (root s0))))
+  (get_input (get_pc (c))) =
+circle_op_2 (root s).
+
+Axiom co_2_def:
+forall (s0 : SE_tree) (s: sym_state),
+is_leaf_state s0 s ->
+conc_ex (circle_op_2 (root s0))
+  (get_input (get_pc s)) =
+(circle_op_2  s).
+
+Axiom co_2_def2:
+forall (A B : SE_tree),
+trees_connect A B ->
+forall c : sym_state,
+  is_leaf_state A c ->
+  conc_ex (circle_op_2 (root A)) (get_input (get_pc c)) =
+  circle_op_2 (root B).
 
 
 Theorem tlist_size: 
@@ -182,6 +315,21 @@ size (tlist :: s) = S (size tlist).
 Proof. intros. induction tlist.
 -simpl;auto.
 -simpl; auto. Qed.
+
+Definition check_eq_prop (B : SE_tree) (c d : sym_state) : Prop :=
+Included ConcState.conc_state (circle_op_2 c) (circle_op_1 (root B) d). 
+
+(*Find leaf c of A such that circle_op_2(c) is subset of circle_op_1(B, d),
+ where d is a leaf of B.*)
+
+Definition fl := SE_tree -> sym_state.
+Axiom find_leaf : fl.
+
+Axiom Prop_3_req: forall (A B : SE_tree) (c : sym_state), 
+(check_eq_prop B (find_leaf A) c ) = True.
+
+
+
 
 
 
@@ -221,7 +369,7 @@ Variable tree_list : SymbolicExec.SE_tree_list.
 
 Axiom tl_size: (size tree_list) >= 2.
 
-(*Expand circle ops*)
+
 Axiom property1 : 
 Included ConcState.conc_state 
 init_conc_states
@@ -234,6 +382,8 @@ Axiom property2: (Intersection ConcState.conc_state (circle_op_2 (root (last_ele
 
 Axiom property3: is_connected tree_list.
 
+Axiom p3: is_connected2 tree_list.
+
 Theorem cio_helper: 
 forall (t : SE_tree_list) (A B s : SE_tree),
 (is_consecutive_in_order A B t)
@@ -243,7 +393,10 @@ destruct t.
 -simpl;auto.
 -simpl. simpl in H. right. assumption. Qed.
 
-
+Axiom connected_elim2: 
+forall (t : SE_tree_list) (s0 s : SE_tree),
+is_connected2 ((t :: s0) :: s)->
+is_connected2 (t :: s0).
 
 
 Theorem connected_elim: 
@@ -261,21 +414,7 @@ apply H.
 *simpl;auto.
 *apply cio_helper. apply H1. Qed.
 
-Axiom base_case: 
-forall s0 s : SE_tree,
-is_connected (([ ] :: s0) :: s) ->
-conc_ex
-  (conc_ex init_conc_states
-     (get_input (get_pc (root s0))))
-  (get_input (get_pc (root s))) =
-circle_op_2 (root s).
 
-Axiom co_2_def:
-forall (s0 : SE_tree) (s: sym_state),
-is_leaf_state s0 s ->
-conc_ex (circle_op_2 (root s0))
-  (get_input (get_pc s)) =
-(circle_op_2  s).
 
 Theorem connected_ends: 
 forall s1 s0 s : SE_tree,
@@ -283,6 +422,15 @@ is_connected ((([] :: s1) :: s0) :: s) -> is_leaf_state s0 (root s).
 Proof. intros. unfold is_connected in H. apply H. 
 -simpl;auto.
 -simpl;auto. Qed.
+
+Axiom bc_helper2: 
+forall s0 s : SE_tree,
+is_connected2 (([ ] :: s0) :: s) ->
+execute_tree_list  (([ ] :: s0) :: s) = 
+conc_ex
+  (conc_ex init_conc_states
+     (get_input (get_pc (root s0))))
+  (get_input (get_pc (root s))).
 
 Theorem bc_helper: 
 forall s0 s : SE_tree,
@@ -307,9 +455,33 @@ rewrite bc_helper.
 *apply connected_ends in H. apply H.
 *auto.
 -auto. Qed.
- 
 
+(*Axiom bcbc : 
+forall (s1 s0 : SE_tree) (c : sym_state),
+is_leaf_state s1 c ->
+execute_tree_list (([ ] :: s1) :: s0)
+= conc_ex (conc_ex init_conc_states (get_input (get_pc (root htop)))) (get_input (get_pc  (root t)))*)
+(*
+Theorem bc22 : forall (s s0 s1 : SE_tree),
+is_connected2 ((([] :: s1) :: s0) :: s) ->
+forall (c : sym_state),
+(is_leaf_state s0 c) ->
+(conc_ex (execute_tree_list (([] :: s1) :: s0))
+  (get_input (get_pc (c))) =
+circle_op_2
+  (root (last_elem ((([] :: s1) :: s0) :: s)))).*)
+(*Proof. intros. pose H as H1. apply connected_elim2 in H1.
+*)
 
+pose bc2 as bc. rewrite bc_helper2.
+*simpl. apply bc. Search "bc".
+
+simpl. apply bc2.
+rewrite bc_helper2.
+- apply bc2.
+*simpl. rewrite co_2_def2.
+rewrite <- exists_elim. rewrite co_2_def2. split. auto.
+*
 
 
 
@@ -351,6 +523,18 @@ forall (x : SE_tree_list) (y z : SE_tree),
 Proof. intros. simpl; auto. Qed.
 
 
+Axiom connection2:
+forall (t : SE_tree_list) (s s0 s1 s2 : SE_tree),
+is_connected2 ((((t :: s2) :: s1) :: s0) :: s) ->
+conc_ex
+  (circle_op_2
+     (root (last_elem (((t :: s2) :: s1) :: s0))))
+  (get_input (get_pc (root s))) =
+circle_op_2
+  (root
+     (last_elem ((((t :: s2) :: s1) :: s0) :: s))).
+
+
 Theorem connection:
 forall (t : SE_tree_list) (s s0 s1 s2 : SE_tree),
 is_connected ((((t :: s2) :: s1) :: s0) :: s) ->
@@ -366,7 +550,31 @@ unfold is_connected in H. apply H.
 -apply size_const_3_helper.
 - apply cio_fundamental. Qed.
 
-
+Theorem etl_con2 : 
+forall t: SE_tree_list,
+is_connected2 t /\ (size t) >= 2 -> 
+execute_tree_list t = 
+(circle_op_2 (root (last_elem t))).
+Proof. intros. destruct H.
+induction t. 
+-inversion H0.
+-destruct t.
+*inversion H0. inversion H2.
+*destruct t.
++rewrite etl_size2_modified. unfold last_elem.
+++apply bc2. apply H.
+++auto.
++destruct t.
+++rewrite etl_size_gt2. 
++++apply bc22. assumption.
++++simpl;auto.
+++rewrite etl_size_gt2.
++++ rewrite IHt. apply connection2.
+assumption.
+++++ apply connected_elim2 in H. assumption.
+++++apply size_const_helper.
++++apply size_const_2_helper.
+Qed.
 
 
 
@@ -409,6 +617,11 @@ Proof. apply etl_con. split.
 -apply property3.
 -apply tl_size.  Qed.
 
+
+Theorem etl2 : execute_tree_list tree_list = (circle_op_2 (root (last_elem tree_list))).
+Proof. apply etl_con2. split.
+-apply p3.
+-apply tl_size. Qed.
 
 
 Theorem sufficiency : 
